---
title: Quiz 6 - More chain rule and differentiation of trigonometric functions
---

## Problem 1
### Question
Differentiate $y = \sin^{-1}(e^{-x}) + \sec^{-1}(e^x)$.

### Solution
$$
\begin{align}
y &= \sin^{-1}(e^{-x}) + \sec^{-1}(e^x) \\
\frac{d}{dx}y &= \frac{d}{dx}\left(\sin^{-1}(e^{-x}) + \sec^{-1}(e^x)\right) \\
&= \frac{1}{\sqrt{1-e^{-2x}}}\frac{d}{dx}e^{-x} + \frac{1}{e^{2x}\sqrt{1-e^{-2x}}}\frac{d}{dx}e^x \\
&= -\frac{e^{-x}}{\sqrt{1-e^{-2x}}} + \frac{e^x}{e^{2x}\sqrt{1-e^{-2x}}} \\
&= -\frac{1}{e^x\sqrt{1-e^{-2x}}} + \frac{1}{e^{x}\sqrt{1-e^{-2x}}} \\
\Aboxed{\frac{d}{dx}y&= 0}
\end{align}
$$

